src/lib/Red2.v
@@ -1,0 +1,177 @@
+From Ltac2 Require Import Ltac2.
+From Ltac2 Require Option Array Ident Control Std Fresh Message.
+
+Ltac2 or t0 t1 :=
+  match! 'True with
+  | True => t0 ()
+  | _ => t1 ()
+  end.
+
+Ltac2 fail () := Control.zero Match_failure.
+
+Ltac2 tcsearch e :=
+  let x := Array.make 1 constr:(tt: unit) in
+  or (fun _ =>
+        let n := Fresh.in_goal ident:(_TC_) in
+        ltac1:(e n|- unshelve evar (n: e);
+               [typeclasses eauto|]) (Ltac1.of_constr e) (Ltac1.of_ident n);
+        Array.set x 0 (Std.eval_unfold [(Std.VarRef n, Std.AllOccurrences)] (Control.hyp n));
+        fail ())
+     (fun _ => Array.get x 0)
+.
+
+Set Default Proof Mode "Classic".
+
+Ltac2 Type flag := [ Break | Continue | Fail ].
+
+(* Internals *)
+Lemma _equal_f (A B : Type) (f g : A -> B)
+      x
+      (EQ: f = g)
+  :
+    f x = g x.
+Proof.
+  subst. apply eq_refl.
+Qed.
+
+Lemma _einit (P Q: Prop)
+      (EQ: P = Q)
+  :
+    Q -> P.
+Proof.
+  subst. apply id.
+Qed.
+
+Ltac2 rec _ctx n :=
+  match! n with
+  | O => apply f_equal
+  | S ?m => apply _equal_f; _ctx m
+  end.
+
+Ltac2 __prw red_tac success :=
+  cbn;
+  tryif (let f := fresh "f" in
+         evar (f:_flag);
+         etransitivity;
+         [red_tac|
+           match goal with
+           | [f0:= ?f1: _flag|- _] =>
+               match f1 with
+               | _continue => subst f; __prw red_tac true
+               | _break => subst f; reflexivity
+               | _fail => fail 2
+               end
+           end])
+  then
+    idtac
+  else
+    match success with
+    | true => reflexivity
+    | false => fail
+    end.
+
+Ltac _prw k0 k1 X :=
+  match X with
+  | O => eapply _einit; [(k0; k1)|]
+  | S ?n => _prw ltac:(k0; _ctx n) k1
+  end.
+
+Ltac _rwb k X :=
+  match X with
+  | O => k
+  | _ => _rwb ltac:(fun f => ltac:(k f || (instantiate (f:=_break); eapply X; fail)))
+  end.
+
+Ltac _rwc k X :=
+  match X with
+  | O => k
+  | _ => _rwc ltac:(fun f => ltac:(k f || (instantiate (f:=_continue); eapply X; fail)))
+  end.
+
+Ltac _rwa k X :=
+  match X with
+  | O => k
+  | (?H, ?_f) => _rwa ltac:(fun f => ltac:(k f || (instantiate (f:=_f); eapply H; fail)))
+  end.
+
+(* Main Tactic *)
+Ltac prw red_tac X := _prw ltac:(idtac) ltac:(__prw red_tac false) X.
+
+Ltac rwbl X := _rwb ltac:(fun f => fail) X.
+Ltac rwcl X := _rwc ltac:(fun f => fail) X.
+Ltac rwal X := _rwa ltac:(fun f => fail) X.
+Ltac rrw X _f := ltac:(fun f => instantiate (f:=_f); eapply X; fail).
+
+Module TUTORIAL.
+  Section FOO.
+    (* Variables *)
+    Variable A B C: Type.
+    Variable a b c d: A.
+    Variable x y z: B.
+    Variable p q: C.
+
+    Variable sim: A -> (nat * B) * C -> nat -> Prop.
+
+    (* First Step: Prove Reduction Lemmas *)
+    Hypothesis foo_red0: a = b.
+    Hypothesis foo_red1: b = c.
+    Hypothesis foo_red2: c = d.
+    Hypothesis foo_red3: x = y.
+    Hypothesis foo_red4: y = z.
+    Hypothesis foo_red5: p = q.
+
+    (* Second Step: Define Reduction Strategy (= red_tac) *)
+    Ltac red_A f := (* f is a flag indicating continue/break/fail. Must set f before return *)
+      ((instantiate (f:=_continue); apply foo_red0; fail) ||
+       (instantiate (f:=_break); apply foo_red1; fail) ||
+       (instantiate (f:=_fail); apply foo_red2; fail)).
+
+    (* We also give more conenient syntax *)
+    Ltac red_A' := (* = red_A *)
+      rwal (foo_red0, _continue)
+           (foo_red1, _break)
+           (foo_red2, _break)
+           0.
+
+    Ltac red_B :=
+      rwcl foo_red3
+           foo_red4
+           0.
+
+    Ltac red_B' f := (* = red_B *)
+      ((instantiate (f:=_continue); apply foo_red3; fail) ||
+       (instantiate (f:=_continue); apply foo_red4; fail)).
+
+    Ltac red_C :=
+      rrw foo_red5 _break.
+
+    Ltac red_C' := (* = red_C *)
+      rwbl
+        foo_red5
+        0.
+
+    Ltac red_C'' f := (* = red_C *)
+      (instantiate (f:=_break); apply foo_red5; fail).
+
+    (* Done. Let's use it! *)
+    Lemma foo: forall (n: nat) (H: sim c ((n, z), q) n),
+        sim a ((n, x), p) n.
+    Proof.
+      intros n H.
+      (* goal = sim a (n, x, p) n *)
+      prw red_B 2 2 1 0.
+      (* prw [red_tac (= red_r)] [l_0 (= 2)] [l_1 (= 2)] [l_2 (= 1)] ... 0 =>
+         - find the right l_0th term x0 (= ((n, x), p)) in the goal
+         - find the right l_1th term x1 (=  (n, x)    ) in the   x0
+         - find the right l_2th term x2 (=      x     ) in the   x1
+         ...
+         - the last argument must be 0. reduce the x2 following _red_r *)
+      (* goal = sim a (n, z, p) n *)
+      prw red_A 3 0.
+      (* goal = sim c (n, z, p) n *)
+      prw red_C 2 1 0.
+      (* goal = sim c (n, z, q) n *)
+      exact H.
+    Qed.
+  End FOO.
+End TUTORIAL.
